update fsub/autosubst2_sctx defs

fsub/autosubst2_sctx/language.sig
@@ -6,12 +6,13 @@ entry : Type
 -- the constructors for typ
 typ_arr : typ -> typ -> typ
 typ_all : typ -> (bind typ in typ) -> typ
+typ_top : typ
 
 -- the constructors for exp
 exp_app  : exp -> exp -> exp
 exp_abs  : typ -> (bind exp in exp) -> exp
 exp_tapp : exp -> typ -> exp
-exp_tabs : (bind typ in exp) -> exp
+exp_tabs : typ -> (bind typ in exp) -> exp
 
 entry_var : typ -> entry
 entry_tvar : typ -> entry
