fsub/autosubst2_sctx/def_extra.v
@@ -1,0 +1,114 @@
+Require Import List.
+
+Require Import common.prop_as_core.
+Require Import common.prop_as_unscoped.
+Require Import fsub.autosubst2_sctx.def_as2.
+
+Import SubstNotations.
+Import UnscopedNotations.
+
+Definition ctx := list entry.
+
+Definition ren_entry (ξ : nat -> nat) (e : entry) : entry :=
+  match e with
+  | entry_var A => entry_var (A ⟨ ξ ⟩)
+  | entry_tvar A => entry_tvar (A ⟨ ξ ⟩)
+  end.
+
+Inductive lookup_tvar : nat -> list entry -> typ -> Prop :=
+| here_tvar A Δ : lookup_tvar 0 ((entry_tvar A) :: Δ) (A ⟨ ↑ ⟩) 
+| skip_var n Δ A B : lookup_tvar n Δ A -> lookup_tvar n (cons (entry_var B) Δ) A
+| there_tvar n Δ A B : lookup_tvar n Δ A -> lookup_tvar (S n) (cons (entry_tvar B) Δ) (A ⟨ ↑ ⟩).
+
+Inductive lookup_var : nat -> list entry -> typ -> Prop :=
+| here_var A Γ : lookup_var 0 ((entry_var A) :: Γ) A 
+| skip_tvar n Γ A B : lookup_var n Γ A -> lookup_var n (cons (entry_tvar B) Γ) (A ⟨ ↑ ⟩)
+| there_var n Γ A B : lookup_var n Γ A -> lookup_var (S n) (cons (entry_var B) Γ) A.
+
+Fixpoint wf_typ Δ A := match A with
+  | typ_var X => exists B, lookup_tvar X Δ B
+  | typ_top => True
+  | typ_arr A B => wf_typ Δ A /\ wf_typ Δ B
+  | typ_all A B => wf_typ Δ A /\ wf_typ ((entry_tvar A) :: Δ) B
+end.
+
+Notation "Δ ⊢ A" := (wf_typ Δ A) (at level 99).
+
+Reserved Notation "Δ ⊢ A <: B" 
+  (at level 99, A at next level, no associativity).
+Inductive subtyping : ctx -> typ -> typ -> Prop :=
+| sub_top Δ A :
+  Δ ⊢ A ->
+  Δ ⊢ A <: typ_top
+| sub_tvar_refl Δ X :
+  Δ ⊢ typ_var X ->
+  Δ ⊢ typ_var X <: typ_var X
+| sub_tvar_bound Δ X A B: 
+  lookup_tvar X Δ A ->
+  Δ ⊢ A <: B ->
+  Δ ⊢ typ_var X <: B
+| sub_arrow Δ A1 A2 B1 B2 : 
+  Δ ⊢ B1 <: A1 ->
+  Δ ⊢ A2 <: B2 ->
+  Δ ⊢ (typ_arr A1 A2) <: (typ_arr B1 B2)
+| sub_all Δ A1 A2 B1 B2
+  (Hwf : Δ ⊢ B1) 
+  (Hsub1 : Δ ⊢ B1 <: A1)
+  (Hsub2 : ((entry_tvar B1) :: Δ) ⊢ A2 <: B2) :
+  Δ ⊢ (typ_all A1 A2) <: (typ_all B1 B2)
+where "Δ ⊢ A <: B" := (subtyping Δ A B).
+
+Reserved Notation "Γ ⊢ t : A" 
+  (at level 99, t at next level, no associativity).
+Inductive typing : ctx -> exp -> typ -> Prop :=
+| typing_var Γ i A :
+  lookup_var i Γ A ->
+  Γ ⊢ (exp_var i) : A
+| typing_abs Γ t A B :
+  Γ ⊢ A ->
+  (entry_var A :: Γ) ⊢ t : B ->
+  Γ ⊢ (exp_abs A t) : (typ_arr A B)
+| typing_app Γ s t A B :
+  Γ ⊢ t : (typ_arr A B) ->
+  Γ ⊢ s : A ->
+  Γ ⊢ (exp_app t s) : B
+| typing_tabs : forall Γ t A B,
+  Γ ⊢ A ->
+  (entry_tvar A :: (map (ren_entry ↑) Γ)) ⊢ t : B ->
+  Γ ⊢ (exp_tabs A t) : (typ_all A B)
+| typing_tapp : forall Γ t A B A' B',
+  Γ ⊢ t : (typ_all A B) ->
+  Γ ⊢ A' <: A ->
+  B' = B [A'..] ->
+  Γ ⊢ exp_tapp t A' : B'
+| typing_sub : forall Γ t A B,
+  Γ ⊢ t : A ->
+  Γ ⊢ A <: B ->
+  Γ ⊢ t : B
+where " Γ ⊢ t : A" := (typing Γ t A).
+
+Definition is_value (t : exp) : Prop :=
+  match t with
+  | exp_abs _ _ => True
+  | exp_tabs _ _ => True
+  | _ => False
+  end.
+
+Reserved Notation "t ⤳ t'" (at level 80).
+Inductive step : exp -> exp -> Prop :=
+| step_beta t s A :
+  is_value s ->
+  exp_app (exp_abs A t) s ⤳ t [typ_var ; scons s exp_var] 
+| step_inst t A B :
+  exp_tapp (exp_tabs A t) B ⤳ t [scons B typ_var; exp_var]
+| step_appl t t' s : 
+  t ⤳ t' -> 
+  exp_app t s ⤳ exp_app t' s
+| step_appr t s s' : 
+  is_value t ->
+  s ⤳ s' -> 
+  exp_app t s ⤳ exp_app t s'
+| step_tapp t t' A : 
+  t ⤳ t' ->
+  exp_tapp t A ⤳ exp_tapp t' A
+where "t ⤳ t'" := (step t t').
